Adding a basic library about pickability.

theories/tiles.v
@@ -3,6 +3,23 @@
 
 Record game_state := {
     length : nat * nat ;
-    state : { x | x < fst length } -> { y | y < fst length } -> bool
+    state : nat -> nat -> bool ;
+    state_out_x : forall x y, x >= fst length -> state x y = false ;
+    state_out_y : forall x y, y >= snd length -> state x y = false ;
+    state_origin : state 0 0 = true
   }.
+
+(** With this definition, we know that there is at least one tile. **)
+Lemma game_state_length_gt_0 : forall st : game_state,
+  fst (length st) <> 0 /\ snd (length st) <> 0.
+Proof.
+  intro st. pose (E := state_origin st).
+  split; intro E0.
+  - rewrite state_out_x in E.
+    + now inversion E.
+    + now rewrite E0; auto.
+  - rewrite state_out_y in E.
+    + now inversion E.
+    + now rewrite E0; auto.
+Qed.
 
