lib/common.v
@@ -1,0 +1,8 @@
+(** Some very basic definitions, already present in quite a lot of libraries. **)
+
+From Coq Require Export Bool.Bool.
+
+Definition decidable P := { P } + { ~ P }.
+
+Coercion is_true : bool >-> Sortclass.
+
